wip porting IncrementWait to new constants style
and generic StateMachineMMIO rather than IncrementWaitMMIO

investigations/bedrock2/IncrementWait/Constants.v
@@ -1,91 +1,10 @@
-Require Import Coq.Lists.List.
 Require Import Coq.Strings.String.
 Require Import Coq.ZArith.ZArith.
-Require Import Coq.Lists.List.
-Require Import bedrock2.Semantics.
-Require Import bedrock2.Syntax.
-Require Import coqutil.Word.Interface.
-Require Import Bedrock2Experiments.Word.
-
-Import ListNotations.
 Local Open Scope string_scope.
-Local Open Scope list_scope.
 
 (* read and write interaction names *)
 Definition READ := "MMIOREAD".
 Definition WRITE := "MMIOWRITE".
 
-(* Core class : defines all the constants *)
-Class constants T :=
-  { VALUE_ADDR : T;
-    STATUS_ADDR : T;
-    STATUS_DONE : T }.
-
-(* Given the string names of all the constants, coerce them to bedrock2
-   expressions with expr.var *)
-Definition constant_vars
-           {names : constants string}
-  : constants expr :=
-  {| VALUE_ADDR := expr.var VALUE_ADDR;
-     STATUS_ADDR := expr.var STATUS_ADDR;
-     STATUS_DONE := expr.var STATUS_DONE;
-  |}.
-
-(* Given the Z values of all the constants, convert them to exprs with
-   expr.literal *)
-Definition constant_literals
-           {vals : constants Z}
-  : constants expr :=
-  {| VALUE_ADDR := expr.literal VALUE_ADDR;
-     STATUS_ADDR := expr.literal STATUS_ADDR;
-     STATUS_DONE := expr.literal STATUS_DONE;
-  |}.
-
-(* Given the Z values of all the constants, convert them to words with
-   word.of_Z *)
-Definition constant_words
-           {width} {word : word width} {word_ok : word.ok word}
-           {vals : constants Z}
-  : constants word :=
-  {| VALUE_ADDR := word.of_Z VALUE_ADDR;
-     STATUS_ADDR := word.of_Z STATUS_ADDR;
-     STATUS_DONE := word.of_Z STATUS_DONE;
-  |}.
-
-(* This instance provide the string name for each constant *)
-Definition constant_names : constants string :=
-  {| VALUE_ADDR := "VALUE_ADDR";
-     STATUS_ADDR := "STATUS_ADDR";
-     STATUS_DONE := "STATUS_DONE";
-  |}.
-
-(* This list includes all the constants and is prepended to functions' argument
-   lists to initialize their environment *)
-Definition globals {T} {consts : constants T} : list T :=
-  [ VALUE_ADDR
-    ; STATUS_ADDR
-    ; STATUS_DONE
-  ].
-
-(* All register addresses *)
-Definition reg_addrs {width} {word : word.word width}
-           {global_values : constants word}
-  : list word.rep := [VALUE_ADDR (*; STATUS_ADDR <-- same addr as VALUE_ADDR, using bit 31 *)].
-
-(* This class includes all the properties the constants must satisfy *)
-Class constants_ok
-      {width} {word : word width} {word_ok : word.ok word}
-      (global_values : constants word) :=
-  { addrs_unique : NoDup reg_addrs;
-    addrs_aligned :
-      Forall (fun w => word.unsigned w mod 4 = 0) reg_addrs;
-    addrs_small :
-      Forall (fun w => word.unsigned w + 4 < 2 ^ 32) reg_addrs;
-    status_flags_unique_and_nonzero :
-      NoDup
-        ((word.of_Z 0)
-           :: (map (fun flag_position => word.slu (word.of_Z 1) flag_position)
-                  [STATUS_DONE]));
-    flags_lt_width : Forall (fun w => word.unsigned w < width)
-                            [STATUS_DONE]
-  }.
+Definition VALUE_ADDR: Z := 16 * 2^10.
+Definition STATUS_ADDR: Z := 16 * 2^10.
