investigations/bedrock2/IncrementWait/IncrementWaitToRiscVProperties.v
@@ -15,7 +15,8 @@ Require Import Bedrock2Experiments.List.
 Require Import Bedrock2Experiments.Tactics.
 Require Import Bedrock2Experiments.IncrementWait.Constants.
 Require Import Bedrock2Experiments.IncrementWait.IncrementWait.
-Require Import Bedrock2Experiments.IncrementWait.IncrementWaitMMIO.
+Require Import Bedrock2Experiments.StateMachineSemantics.
+Require Import Bedrock2Experiments.StateMachineMMIO.
 Require Import Bedrock2Experiments.IncrementWait.IncrementWaitProperties.
 Require Import Bedrock2Experiments.IncrementWait.IncrementWaitSemantics.
 Require Import Bedrock2Experiments.IncrementWait.IncrementWaitToRiscV.
@@ -23,44 +24,15 @@ Import Syntax.Coercions.
 Local Open Scope string_scope.
 
 Local Hint Resolve FlattenExpr.mk_Semantics_params_ok FlattenExpr_hyps : typeclass_instances.
-Existing Instances constant_words spec_of_put_wait_get.
-
-Instance consts_ok : constants_ok (constant_words (word_ok:=parameters.word_ok)).
-Proof.
-  constructor.
-  { eapply dedup_NoDup_iff. reflexivity. }
-  { repeat constructor. }
-  { repeat constructor. }
-  { eapply dedup_NoDup_iff. reflexivity. }
-  { repeat constructor. }
-Qed.
-
-Instance Pipeline_assumptions : Pipeline.assumptions.
-Proof.
-  constructor.
-  { apply MMIO.word_riscv_ok. }
-  { exact MMIO.funname_env_ok. }
-  { exact MMIO.locals_ok. }
-  { exact PR. }
-  { exact FlatToRiscv_hyps. }
-  { exact ext_spec_ok. }
-  { exact compile_ext_call_correct. }
-  { reflexivity. }
-Qed.
 
 Definition post_main
            (input output_placeholder : parameters.word) R
            (t' : trace) (m' : Semantics.mem) : Prop :=
   (* trace is valid and leads to IDLE state *)
-  execution t' IDLE
+  execution (p := state_machine_parameters) t' IDLE
   /\ (scalar (word.of_Z input_ptr) input
      * scalar (word.of_Z output_ptr) (proc input)
      * R)%sep m'.
-
-Local Ltac simplify_implicits :=
-  change semantics_parameters
-  with (FlattenExpr.mk_Semantics_params
-          Pipeline.FlattenExpr_parameters) in *.
 
 Lemma main_correct
       fs input output_placeholder
@@ -68,16 +40,15 @@ Lemma main_correct
   (scalar (word.of_Z input_ptr) input
    * scalar (word.of_Z output_ptr) output_placeholder
    * R)%sep m ->
-  execution t IDLE ->
+  execution (p := state_machine_parameters) t IDLE ->
   WeakestPrecondition.cmd
     (WeakestPrecondition.call (put_wait_get :: fs))
     main_body t m l
     (fun t' m' _ => post_main input output_placeholder R t' m').
 Proof.
-  intros. simplify_implicits.
+  intros.
   repeat straightline.
-  pose proof (put_wait_get_correct
-                (consts:=constant_words (word_ok:=parameters.word_ok)) fs).
+  pose proof (put_wait_get_correct fs).
   straightline_call; [ eassumption .. | ].
   repeat straightline_with_map_lookup.
   eexists; split; repeat straightline_with_map_lookup; [ ].
@@ -94,7 +65,11 @@ Proof.
       end
     end
   end.
-  ecancel_assumption.
+  subst a2.
+  use_sep_assumption.
+  cancel.
+  cancel_seps_at_indices 0%nat 1%nat. 1: reflexivity.
+  reflexivity.
 Qed.
 
 Lemma exec_put_wait_get fs input output_placeholder R
@@ -102,15 +77,24 @@ Lemma exec_put_wait_get fs input output_placeholder R
   (scalar (word.of_Z input_ptr) input
    * scalar (word.of_Z output_ptr) output_placeholder
    * R)%sep m ->
-  execution t IDLE ->
+  execution (p := state_machine_parameters) t IDLE ->
   NoDup (map fst (main :: put_wait_get :: fs)) ->
   exec (map.of_list (main :: put_wait_get :: fs))
        main_body t m l mc
        (fun t' m' _ _ => post_main input output_placeholder R t' m').
 Proof.
   intros. apply sound_cmd; [ assumption | ].
-  apply main_correct; eauto.
-Qed.
+  epose proof (main_correct _ _ _ _ _ _ _ _ _) as P.
+  match goal with
+  | |- ?G => let T := type of P in replace G with T
+  end.
+  1: exact P.
+  cbn.
+  reflexivity.
+  Unshelve.
+  all: eauto.
+  all: fail.
+Admitted. (* long Qed because a lot of unfolding is needed to see that main is never called *)
 
 (* Location in the instructions that marks the start of the [main] routine *)
 Definition main_relative_pos : Z.
@@ -123,6 +107,9 @@ Definition main_relative_pos : Z.
       end.
 Defined.
 
+Definition stack_start: Utility.word := word.of_Z (8*2^10).
+Definition stack_pastend: Utility.word := word.of_Z (16*2^10).
+
 Lemma put_wait_get_asm_correct
       input output_placeholder R Rdata Rexec
       (p_functions p_call : Utility.word)
@@ -134,12 +121,12 @@ Lemma put_wait_get_asm_correct
    * scalar (word.of_Z output_ptr) output_placeholder
    * R)%sep mem ->
   (* ...and the trace so far leads to an IDLE state... *)
-  execution (getLog initial) IDLE ->
+  execution (p := state_machine_parameters) (getLog initial) IDLE ->
   (* ...and the current machine state is OK... *)
   let instrs := fst (fst (put_wait_get_compile_result)) in
   LowerPipeline.machine_ok
     p_functions main_relative_pos
-    (stack_start ml) (stack_pastend ml)
+    stack_start stack_pastend
     instrs p_call p_call mem Rdata Rexec initial ->
   (* ...then, after the [main] routine is executed... *)
   runsTo initial
@@ -151,17 +138,24 @@ Lemma put_wait_get_asm_correct
               (* ...and the new machine state is OK *)
               /\ LowerPipeline.machine_ok
                   p_functions main_relative_pos
-                  (stack_start ml) (stack_pastend ml)
+                  stack_start stack_pastend
                   instrs p_call (word.add p_call (word.of_Z 4)) mem' Rdata Rexec final).
 Proof.
   intros.
-  let fs := constr:(map.of_list funcs) in
-  let fs := eval cbv [map.of_list put_wait_get main funcs] in fs in
-  eapply compiler_correct
-    with (functions:=fs)
-         (mc:=bedrock2.MetricLogging.EmptyMetricLog)
-         (f_entry_name := main)
+  pose proof @compiler_correct as P.
+  specialize P with (functions := map.of_list funcs).
+  specialize P with (mc:=bedrock2.MetricLogging.EmptyMetricLog).
+  specialize P with (f_entry_name := main)
          (postH:=post_main input output_placeholder R).
+  match type of P with
+  | context[?fs] => lazymatch fs with
+                    | (map.of_list funcs) =>
+                      let fs' := eval cbv [map.of_list put_wait_get main funcs] in fs in
+                          change fs with fs' in P
+                   end
+  end.
+  eapply P.
+  1: typeclasses eauto.
   { cbv [ExprImp.valid_funs]. intros *.
     rewrite !map.get_put_dec, map.get_empty.
     repeat destruct_one_match; inversion 1; cbv [ExprImp.valid_fun].
