investigations/bedrock2/IncrementWait/IncrementWait.v
@@ -13,11 +13,11 @@ Local Open Scope Z_scope.
 Local Open Scope list_scope.
 
 Section Impl.
-  Local Existing Instances constant_names constant_vars.
 
   (* Notations for small constants *)
   Local Notation "0" := (expr.literal 0) (in custom bedrock_expr).
   Local Notation "1" := (expr.literal 1) (in custom bedrock_expr).
+  Local Notation "31" := (expr.literal 31) (in custom bedrock_expr).
 
   (* Sets the VALUE register, waits for a DONE status, reads the result, and
      returns it. Assumes the circuit is in IDLE state at the start. *)
@@ -29,13 +29,13 @@ Section Impl.
     (* temporary variables *)
     let status := "status" in
     ("put_wait_get",
-     (globals ++ [input], [out], bedrock_func_body:(
+     ([input], [out], bedrock_func_body:(
         (* write input value *)
         output! WRITE (VALUE_ADDR, input) ;
         (* initialize status to 0 *)
         status = 0 ;
         (* wait for status to be DONE *)
-        while ((status & (1 << STATUS_DONE)) == 0) {
+        while ((status & (1 << 31)) == 0) {
           io! status = READ ( STATUS_ADDR )
         };
         (* read the value *)
